Add typechecking of values/completeness proofs

theories/Decide.v
@@ -10,6 +10,7 @@ Module Import SpecNotations.
   Infix "*" := t_prod.
 
   Notation "Γ ⊢ E 'in' t" := (judge_E Γ E t) (at level 90).
+  Notation "⊢ v 'in' t" := (judge_v v t) (at level 90).
 End SpecNotations.
 
 Definition eq_type (x y: type): {x = y} + {x <> y}.
@@ -17,12 +18,16 @@ Proof.
   decide equality.
 Defined.
 
-Function typecheck (Γ: environment) (e: context): option (environment * type) :=
-  match e with
+Function typecheck (Γ: environment) (E: context): option (environment * type) :=
+  match E with
   | E_var x =>
       if Env.find x Γ is Some t
       then
-        Some (Map.one x t, t)
+        if Env.is_empty (Env.remove x Γ)
+        then
+          Some (Map.one x t, t)
+        else
+          None
       else
         None
   | E_all x t1 E =>
@@ -57,14 +62,136 @@ Function typecheck (Γ: environment) (e: context): option (environment * type) :
     %list.
 
 Theorem typecheck_sound:
-  forall Γ e Δ t, typecheck Γ e = Some (Δ, t) -> Δ ⊢ e in t.
+  forall Γ E Δ t, typecheck Γ E = Some (Δ, t) -> Δ ⊢ E in t.
 Proof.
-  intros Γ e.
-  functional induction (typecheck Γ e).
+  intros Γ E.
+  functional induction (typecheck Γ E).
   all: cbn.
   all: intros ? ? p.
   all: inversion p.
   all: subst.
-  all: try econstructor.
+  all: econstructor.
   all: eauto.
 Qed.
+
+Theorem typecheck_complete:
+  forall E Γ t, Γ ⊢ E in t -> forall Δ, typecheck Δ E = Some (Γ, t).
+Proof.
+  intros ? ? ? p.
+  induction p.
+  all: cbn.
+  all: intros ?.
+  - admit.
+  - rewrite (IHp _).
+    unfold find in H.
+    rewrite H.
+    destruct (eq_type t1 t1).
+    2: contradiction.
+    reflexivity.
+  - rewrite (IHp1 _).
+    rewrite (IHp2 _).
+    destruct (eq_type t1 t1).
+    2: contradiction.
+    reflexivity.
+Admitted.
+
+
+Function typeof (v: term): option type :=
+  match v with
+  | v_tt => Some t_unit
+  | v_fst v =>
+      if typeof v is Some (t0 * _)
+      then
+        Some t0
+      else
+        None
+  | v_snd v =>
+      if typeof v is Some (_ * t1)
+      then
+        Some t1
+      else
+        None
+  | v_fanout v0 v1 =>
+      if typeof v0 is Some t0
+      then
+        if typeof v1 is Some t1
+        then
+          Some (t0 * t1)
+        else
+          None
+      else
+        None
+  end.
+
+Theorem typeof_sound:
+  forall v t, typeof v = Some t -> ⊢ v in t.
+Proof.
+  intros v.
+  functional induction (typeof v).
+  all: cbn.
+  all: intros ? p.
+  all: inversion p.
+  all: subst.
+  all: econstructor.
+  all: eauto.
+Qed.
+
+Theorem typeof_complete:
+  forall v t, ⊢ v in t -> typeof v = Some t.
+Proof.
+  intros ? ? p.
+  induction p.
+  all: cbn.
+  all: try (destruct (typeof v) as [[]|]).
+  all: try (destruct (typeof v1)).
+  all: try (destruct (typeof v2)).
+  all: try inversion IHp.
+  all: subst.
+  all: try inversion IHp1.
+  all: subst.
+  all: try inversion IHp2.
+  all: subst.
+  all: reflexivity.
+Qed.
+
+Definition E_of_t t := { E | Env.empty _ ⊢ E in t }.
+Definition v_of_t t := { v | ⊢ v in t }.
+
+Definition v_tc v: if typeof v is Some t
+                   then
+                     v_of_t t
+                   else
+                     unit.
+Proof.
+  destruct (typeof v) eqn:q.
+  2: apply tt.
+  exists v.
+  apply typeof_sound.
+  auto.
+Defined.
+
+Lemma is_empty_sound (Γ: Map.map type): Env.is_empty Γ = true -> Γ = Env.empty _.
+Proof.
+  admit.
+Admitted.
+
+Definition E_tc E: if typecheck (Env.empty _) E is Some (Γ, t)
+                   then
+                     if Env.is_empty Γ
+                     then
+                       E_of_t t
+                     else
+                       unit
+                   else
+                     unit.
+Proof.
+  destruct (typecheck (Env.empty _) E) as [[Γ t]|] eqn:q1.
+  2: apply tt.
+  destruct (Env.is_empty Γ) eqn:q2.
+  2: apply tt.
+  exists E.
+  apply (typecheck_sound (Env.empty _) E).
+  rewrite q1.
+  rewrite (is_empty_sound _ q2).
+  reflexivity.
+Defined.
